fall back to rule application proofs for Bellman_Ford.thy

example/Bellman_Ford.thy
@@ -19,7 +19,7 @@ fun bf :: "nat\<times>nat \<Rightarrow> int" where
     fold
     . (min)
     . (map
-        . (\<lambda>i. plus . (W . i . j) . (bf (k, i)))
+        . (\<lambda>i. plus . (W i j) . (bf (k, i)))
         . (upt . 0 . n))
     . (bf (k, j))"
 thm bf.simps
@@ -31,7 +31,7 @@ fun bf\<^sub>T :: "nat\<times>nat \<Rightarrow>\<^sub>T int" where
     \<langle>fold\<^sub>T\<rangle>\<^sub>T
     .\<^sub>T \<langle>min\<^sub>T\<rangle>\<^sub>T
     .\<^sub>T (\<langle>map\<^sub>T\<rangle>\<^sub>T
-      .\<^sub>T \<langle>\<lambda>i. \<langle>plus\<^sub>T\<rangle>\<^sub>T .\<^sub>T (\<langle>\<lambda>\<^sub>T i j. W i j\<rangle>\<^sub>T .\<^sub>T \<langle>i\<rangle>\<^sub>T .\<^sub>T \<langle>j\<rangle>\<^sub>T) .\<^sub>T (bf\<^sub>T (k, i))\<rangle>\<^sub>T
+      .\<^sub>T \<langle>\<lambda>i. \<langle>plus\<^sub>T\<rangle>\<^sub>T .\<^sub>T \<langle>W i j\<rangle>\<^sub>T .\<^sub>T (bf\<^sub>T (k, i))\<rangle>\<^sub>T
       .\<^sub>T (\<langle>upt\<^sub>T\<rangle>\<^sub>T .\<^sub>T \<langle>0\<rangle>\<^sub>T .\<^sub>T \<langle>n\<rangle>\<^sub>T))
     .\<^sub>T (bf\<^sub>T (k, j))"
 term 0 (**)
@@ -73,7 +73,7 @@ lemma bf_inductS':
    \<rbrakk> \<Longrightarrow> bf.consistentS op = (bf (x::nat\<times>nat)) (bf\<^sub>T x)"
   unfolding rel_prod.simps rel_fun_def K_def by (simp add: bf_inductS)
   term 0 (**)
-*)
+
 lemma bf_inductS_l:
   "\<lbrakk>\<And>j. bf.consistentS op = (bf (0, j)) (bf\<^sub>T (0, j));
     \<And>k j. \<lbrakk>(op = ===> bf.consistentS op =) (\<lambda>i'. bf (k, i')) (\<lambda>i'. bf\<^sub>T (k, i'));
@@ -81,22 +81,16 @@ lemma bf_inductS_l:
            \<rbrakk> \<Longrightarrow> bf.consistentS op = (bf (Suc k, j)) (bf\<^sub>T (Suc k, j))
    \<rbrakk> \<Longrightarrow> bf.consistentS op = (bf (x::nat\<times>nat)) (bf\<^sub>T x)"
   unfolding rel_fun_def by (metis bf_inductS)
-
+*)
 term 0 (**)
 
 lemma "bf.consistentDP bf\<^sub>T"
-  apply (rule bf.consistentDP_intro, induct_tac rule: bf_inductS_l, unfold bf\<^sub>T.simps; rule bf.consistentS_checkmem, unfold bf.simps)
-  subgoal premises prems[transfer_rule] by transfer_prover
-  subgoal
-    (*
-    thm bf.fun_app_lifted_transfer[THEN rel_funD, THEN rel_funD]
-    apply (rule bf.fun_app_lifted_transfer[THEN rel_funD, THEN rel_funD, where ?R0.2="op ="])
-    subgoal
-      apply (rule bf.fun_app_lifted_transfer[THEN rel_funD, THEN rel_funD, where ?R0.2="op ="])
-      subgoal
-        apply (rule bf.fun_app_lifted_transfer[THEN rel_funD, THEN rel_funD])
-          apply (rule bf.return_transfer[THEN rel_funD])
-*)
+  apply (rule bf.consistentDP_intro, induct_tac rule: bf_inductS, unfold bf\<^sub>T.simps; rule bf.consistentS_checkmem, unfold bf.simps)
+  subgoal premises prems[transfer_rule]
+    apply (rule bf.return_transfer[THEN rel_funD])
+    apply (simp only:; fail)
+    done
+  subgoal premises prems
     apply (rule bf.fun_app_lifted_transfer[THEN rel_funD, THEN rel_funD])
      apply (rule bf.fun_app_lifted_transfer[THEN rel_funD, THEN rel_funD])
       apply (rule bf.fun_app_lifted_transfer[THEN rel_funD, THEN rel_funD])
@@ -115,32 +109,18 @@ lemma "bf.consistentDP bf\<^sub>T"
         apply (rule bf.return_transfer[THEN rel_funD])
         apply (rule bf.plus_transfer[])
        apply (rule bf.return_transfer[THEN rel_funD])
-       apply (simp only:)
-      
-    oops
-      lemma "\<And>x. "
-      
-term 0 (*
-                        apply transfer_step
-                        apply transfer_step
-                        apply transfer_step
-                        apply transfer_step
-                        apply transfer_step
-                        apply transfer_step
-                        apply transfer_step
-                        apply transfer_step
-                        apply transfer_step
-                        apply transfer_step
-                        apply transfer_step
-                        apply transfer_step
-                        apply transfer_step
-    thm prems(3)
-      supply [transfer_rule] = prems(3)
-                        apply transfer_step
-      apply transfer_step
-      
-      thm prems
-      (* going wrong here *)
-      (* bf\<^sub>T (Pair k i) should be proved directly by prems(1) rather than be separated *)
-    oops
+       apply (simp only:; fail)
+      apply (simp only: prems; fail)
+     apply (rule bf.fun_app_lifted_transfer[THEN rel_funD, THEN rel_funD])
+      apply (rule bf.fun_app_lifted_transfer[THEN rel_funD, THEN rel_funD])
+       apply (rule bf.return_transfer[THEN rel_funD])
+    apply (rule bf.upt_transfer[])
+    apply (rule bf.return_transfer[THEN rel_funD])
+    apply (simp only:; fail)
+    apply (rule bf.return_transfer[THEN rel_funD])
+     apply (simp only:; fail)
+    apply (simp only: prems; fail)
+    done
+  done
+end
 end
